modules/verify/src/main/scala/specrest/verify/z3/Backend.scala
@@ -13,6 +13,7 @@ import com.microsoft.z3.DatatypeSort
 import com.microsoft.z3.Expr as Z3AstExpr
 import com.microsoft.z3.FuncDecl
 import com.microsoft.z3.Model
+import com.microsoft.z3.SeqExpr
 import com.microsoft.z3.Sort
 import com.microsoft.z3.Status
 import specrest.ir.VerifyError
@@ -143,6 +144,8 @@ private def registerSort(ctx: Context, map: mutable.Map[String, Sort], s: Z3Sort
       registerSort(ctx, map, elem)
     case Z3Sort.OptionOf(elem) =>
       registerSort(ctx, map, elem)
+    case Z3Sort.SeqOf(elem) =>
+      registerSort(ctx, map, elem)
     case _ => ()
 
 private def resolveSort(ctx: Context, sortMap: mutable.Map[String, Sort], s: Z3Sort): Sort =
@@ -164,6 +167,8 @@ private def resolveSort(ctx: Context, sortMap: mutable.Map[String, Sort], s: Z3S
         Z3Sort.key(s),
         optionSortFor(ctx, sortMap, resolveSort(ctx, sortMap, elem))
       )
+    case Z3Sort.SeqOf(elem) =>
+      sortMap.getOrElseUpdate(Z3Sort.key(s), ctx.mkSeqSort(resolveSort(ctx, sortMap, elem)))
     case Z3Sort.Str => ctx.getStringSort
 
 @SuppressWarnings(Array("org.wartremover.warts.AsInstanceOf"))
@@ -287,6 +292,16 @@ private object Backend:
       optionSortFor(rctx.ctx, rctx.sortMap, v.getSort).getConstructors()(1).apply(v)
     case Z3Expr.StrLit(s, _) =>
       rctx.ctx.mkString(s)
+    case Z3Expr.SeqLit(elemSort, members, _) =>
+      val elemZ   = resolveSort(rctx.ctx, rctx.sortMap, elemSort)
+      val seqSort = rctx.ctx.mkSeqSort(elemZ)
+      val empty   = rctx.ctx.mkEmptySeq(seqSort).asInstanceOf[SeqExpr[Sort]]
+      members.foldLeft[SeqExpr[Sort]](empty): (acc, m) =>
+        val unit =
+          rctx.ctx.mkUnit(renderExpr(rctx, m).asInstanceOf[Z3AstExpr[Sort]]).asInstanceOf[SeqExpr[
+            Sort
+          ]]
+        rctx.ctx.mkConcat(acc, unit)
 
   def renderBool(rctx: RenderCtx, e: Z3Expr): BoolExpr =
     renderExpr(rctx, e).asInstanceOf[BoolExpr]
